Setlec/Cached/CoreNC.lean
@@ -80,7 +80,8 @@ def structEtaCertWithNC (r : CoreFnsI) (fe : FEnv) (depth : Nat)
                 targs.length = cnP ∧
                 us'.length = cvT.levelParams.length ∧
                 cvc.levelParams = cvT.levelParams ∧
-                (cvT.type.stripPis cnP).isSome = true then do
+                (cvT.type.stripPis cnP).isSome = true ∧
+                (towerSlotsAllF fe Tn cnF || recSlotsAllF fe Tn cnF) = true then do
               if ← liftFueled "level comparison"
                   (← isEquivListLM us us') then do
                 if ← defEqListI r fe depth (aargs.take cnP) targs then do
